Refinery/Ctx/Semantics.lean
@@ -322,10 +322,16 @@ theorem Ctx?.Wk.den_comp_drop {Γ Δ : Ctx? α} (ρ : Γ.Wk Δ) [hΔ : Δ.del]
   := have _ := hΔ.wk ρ; M.drop_aff ⊥ _
 
 @[simp]
-theorem Ctx?.PWk.den_refl {Γ : Ctx? α} : (Ctx?.PWk.refl Γ).den (C := C) = 𝟙 (g⟦ Γ ⟧) := by
+theorem Ctx?.PWk.den_refl {Γ : Ctx? α} : (refl Γ).den (C := C) = 𝟙 (g⟦ Γ ⟧) := by
   induction Γ <;> simp [*] <;> rfl
 
-@[simp]
+theorem Ctx?.PWk.den_single {Γ : Ctx? α} {v w : Var? α} (h : v ≤ w) :
+  ((refl Γ).cons h).den (C := C) = _ ◁ h.den := by simp
+
+theorem Ctx?.PWk.den_double {Γ : Ctx? α} {v w v' w': Var? α} (h : v ≤ w) (h' : v' ≤ w')
+  : (((refl Γ).cons h).cons h').den (C := C) = (_ ◁ h.den) ▷ _ ≫ _ ◁ h'.den
+    := by simp [tensorHom_def]
+
 theorem Ctx?.PWk.den_comp {Γ Δ Ξ : Ctx? α} (ρ : Γ.PWk Δ) (ρ' : Δ.PWk Ξ)
   : ρ.den ≫ ρ'.den = (ρ.comp ρ').den (C := C)
   := by rw [<-ρ.den_toWk, <-ρ'.den_toWk, Wk.den_comp, <-PWk.comp_toWk, den_toWk]
